有三个实数 $a,b,c$ 满足
$abc = -1$,
$a + b + c = 4$
且:
$$
{{a} \over {a ^ 2 - 3a - 1}} + 
{{b} \over {b ^ 2 - 3b - 1}} + 
{{c} \over {c ^ 2 - 3c - 1}} =
{4 \over 9}
$$
求
$a ^ 2 + b ^ 2 + c ^ 2$
的值。




$abc = -1$ 

<=> 

${a ^ 2 - 3a - 1} = a ^ 2 - 3a + abc = a(a - 3 + bc)$

$d$



$$ 
	{1 \over a - 3 + bc} + {1 \over b - 3 + ac} + {1 \over c - 3 + ab} = {4 \over 9}
$$



-----------------------------------------------------------------------------------------------------------------------------------------------------------------------------------------------------------------------------------------------------------------------------------------------------------------

$$
	\sum _{i = 1} ^ n x_i ^ 2 = a
$$

求

$$
	\max \sum _{i = 1} ^ {n - 1} \sum _{j = i + 1} ^ n (x_i - x_j) ^ 2
$$

$$
	原式 = (n - 1) \sum _{i = 1} ^ {n} x_i ^ 2 - 2\sum _{i = 1} ^ {n - 1} \sum _{j = i + 1} ^ n x_i x_j\\
	= (n - 1)a + \sum _{i = 1} ^ {n - 1} \sum _{j = i + 1} ^ n -2x_i x_j
$$


$$
	-2ab \leq a ^ 2 + b ^ 2\\
	max_{-2ab} = a ^ 2 + b ^ 2\\
	max_{原式} = (n - 1)a + \sum _{i = 1} ^ {n - 1} \sum _{j = i + 1} ^ n (x_i ^ 2 + x_j ^ 2)\\
	=(n - 1)a + (n - 1)\sum_{i = 1} ^ n x_i
$$

$$
	(n - 1)(a + \sqrt {an})
$$
-----

$$
	x + y + z = 5\\
	(x + y + z) ^ 2 = 25\\
	x ^ 2 + y ^ 2 + z ^ 2 + 2xy + 2yz + 2xz = 25\\
	xy + yz + xz = 3\\
	x ^ 2 + y ^ 2 + z ^ 2 = 19\\
	max_z = \sqrt {19}
$$

---

$$
	z_1 = {{5 + \sqrt {7}} \over {3}},\\
	z_2 = {{5 - \sqrt {7}} \over {3}}.

$$

$$
	y = {{x} \over {x - 4}}
$$

$$
	x + y = {{x} \over {x - 4}} + x
		  = 1 + {4 \over x - 4} + x - 4 + 4
		  \geq 5 + 4
$$

当且仅当 $x - 4 = {4 \over x - 4}$ 时等号成立

解得 $x_1 = 6, x_2 = 2$

当 $x = 2$ 时, $y = -2$ (舍去)

$$

\sqrt{2 * ({1 + \sqrt 3 \over 2}) ^ 2} = \sqrt{2 * {2 + \sqrt 3 \over 2}} = \sqrt {2 + \sqrt 3}

$$

$$

\sqrt{2 * ({1 + \sqrt 3 \over 2}) ^ 2} = \sqrt 2 * {1 + \sqrt 3 \over 2} = {\sqrt 2 + \sqrt 6 \over 2}

$$

$$ 

\sqrt {a + \sqrt b} （a, b \in Q 且 a \neq 0, b \neq 0)

$$
当 $ \sqrt{ a ^ 2 - b } \in Q$时


$$ 

n = \prod _{i = 1} ^ {k} {p_i} ^ {a_i}

$$
$$

 \phi(n) = 
 \prod _{i = 1} ^ k (p_i - 1) \cdot p_i ^ {a_i-1}
 =n \prod _{i = 1} ^ {k} {p_i - 1 \over p_i}
$$
x <= 3/2a
x > -2/3a
-2/3a < x <= 3/2a
0 3
-2/3 a <= 0
3/2a >= 4


---
$$
ax + by + c = 0
y = kx + b
y = k(x - x_0) + y_0

